theories/TRAKHTENBROT/discrete.v
@@ -30,9 +30,11 @@ Section discrete_quotient.
       is decidable and thus we can quotient the model under this bisim obtaining
       a discrete model which is "equivalent" *)
 
-  Variables (Σ : fo_signature) 
-            (HΣs : finite_t (syms Σ))
-            (HΣr : finite_t (rels Σ))
+  Variables (Σ : fo_signature)
+            (ls : list (syms Σ))
+            (lr : list (rels Σ))
+            (*HΣs : finite_t (syms Σ)*)
+            (*HΣr : finite_t (rels Σ)*)
             (X : Type) (M : fo_model Σ X)  
             (fin : finite_t X) 
             (dec : fo_model_dec M)
@@ -43,8 +45,8 @@ Section discrete_quotient.
   (** Construction of the greatest fixpoint of the following operator *)
 
   Let fom_op R x y :=
-       (forall s (v : vec _ (ar_syms Σ s)) p, R (fom_syms M s (v[x/p])) (fom_syms M s (v[y/p]))) 
-    /\ (forall s (v : vec _ (ar_rels Σ s)) p, fom_rels M s (v[x/p]) <-> fom_rels M s (v[y/p])).
+       (forall s, In s ls -> forall (v : vec _ (ar_syms Σ s)) p, R (fom_syms M s (v[x/p])) (fom_syms M s (v[y/p]))) 
+    /\ (forall s, In s lr -> forall (v : vec _ (ar_rels Σ s)) p, fom_rels M s (v[x/p]) <-> fom_rels M s (v[y/p])).
 
   Let fom_op_mono R T : (forall x y, R x y -> T x y) -> (forall x y, fom_op R x y -> fom_op T x y).
   Proof. intros ? ? ? []; split; intros; auto. Qed. 
@@ -58,9 +60,9 @@ Section discrete_quotient.
   Let fom_op_trans R x z : (exists y, fom_op R x y /\ fom_op R y z)
                         -> fom_op (fun x z => exists y, R x y /\ R y z) x z.
   Proof.
-    intros (y & H1 & H2); split; intros s v p.
-    + exists (fom_syms M s (v[y/p])); split; [ apply H1 | apply H2 ].
-    + transitivity (fom_rels M s (v[y/p])); [ apply H1 | apply H2 ].
+    intros (y & H1 & H2); split; intros s Hs v p.
+    + exists (fom_syms M s (v[y/p])); split; [ apply H1 | apply H2 ]; auto.
+    + transitivity (fom_rels M s (v[y/p])); [ apply H1 | apply H2 ]; auto.
   Qed.
 
   Reserved Notation "x ≡ y" (at level 70, no associativity).
@@ -77,11 +79,11 @@ Section discrete_quotient.
   Let fom_eq_fix x y : fom_op fom_eq x y <-> x ≡ y.
   Proof. 
     apply gfp_fix; auto; clear x y.
-    intros f Hf x y H; split; intros s v p.
+    intros f Hf x y H; split; intros s Hs v p.
     + intros n.
       generalize (H n); intros (H1 & H2).
-      apply H1.
-    + apply (H 0).
+      apply H1; auto.
+    + apply (H 0); auto.
   Qed.
 
   (** We build the greatest bisimulation which is an equivalence 
@@ -98,19 +100,19 @@ Section discrete_quotient.
 
   (* It is a congruence wrt to the model *)
 
-  Fact fom_eq_syms x y s v p : x ≡ y -> fom_syms M s (v[x/p]) ≡ fom_syms M s (v[y/p]).
+  Fact fom_eq_syms x y s v p : In s ls -> x ≡ y -> fom_syms M s (v[x/p]) ≡ fom_syms M s (v[y/p]).
   Proof. intros; apply fom_eq_fix; auto. Qed. 
     
-  Fact fom_eq_rels x y s v p : x ≡ y -> fom_rels M s (v[x/p]) <-> fom_rels M s (v[y/p]).
+  Fact fom_eq_rels x y s v p : In s lr -> x ≡ y -> fom_rels M s (v[x/p]) <-> fom_rels M s (v[y/p]).
   Proof. intros; apply fom_eq_fix; auto. Qed.
 
   Hint Resolve fom_eq_refl fom_eq_sym fom_eq_trans fom_eq_syms fom_eq_rels.
 
-  Theorem fom_eq_syms_full s v w : (forall p, v#>p ≡ w#>p) -> fom_syms M s v ≡ fom_syms M s w.
-  Proof. apply map_vec_pos_equiv; eauto. Qed.
+  Theorem fom_eq_syms_full s v w : In s ls -> (forall p, v#>p ≡ w#>p) -> fom_syms M s v ≡ fom_syms M s w.
+  Proof. intro; apply map_vec_pos_equiv; eauto. Qed.
 
-  Theorem fom_eq_rels_full s v w : (forall p, v#>p ≡ w#>p) -> fom_rels M s v <-> fom_rels M s w.
-  Proof. apply map_vec_pos_equiv; eauto; tauto. Qed.
+  Theorem fom_eq_rels_full s v w : In s lr -> (forall p, v#>p ≡ w#>p) -> fom_rels M s v <-> fom_rels M s w.
+  Proof. intro; apply map_vec_pos_equiv; eauto; tauto. Qed.
 
   Hint Resolve finite_t_vec finite_t_pos. 
 
@@ -124,8 +126,10 @@ Section discrete_quotient.
     apply gfp_decidable; auto.
     intros R HR x y.
     apply (fol_bin_sem_dec fol_conj).
-    + do 3 (apply (fol_quant_sem_dec fol_fa); auto; intros).
-    + do 3 (apply (fol_quant_sem_dec fol_fa); auto; intros).
+    + apply forall_list_sem_dec; intros.
+      do 2 (apply (fol_quant_sem_dec fol_fa); auto; intros).
+    + apply forall_list_sem_dec; intros.
+      do 2 (apply (fol_quant_sem_dec fol_fa); auto; intros).
       apply (fol_bin_sem_dec fol_conj); 
         apply (fol_bin_sem_dec fol_imp); auto.
   Qed.
@@ -167,20 +171,20 @@ Section discrete_quotient.
             { i : X -> pos n &
               { j : pos n -> X |
                   (forall x, i (j x) = x)
-               /\ (forall s v, i (fom_syms M s v) = fom_syms Md s (vec_map i v))
-               /\ (forall s v, fom_rels M s v <-> fom_rels Md s (vec_map i v))
+               /\ (forall s v, In s ls -> i (fom_syms M s v) = fom_syms Md s (vec_map i v))
+               /\ (forall s v, In s lr -> fom_rels M s v <-> fom_rels Md s (vec_map i v))
                  } } } } }.
     Proof.
       exists n, Md; exists.
       { intros x y; simpl; apply dec. }
       exists cls, repr; msplit 2; auto.
-      + intros s v; simpl.
+      + intros s v Hs; simpl.
         apply E2.
-        apply fom_eq_syms_full.
+        apply fom_eq_syms_full; auto.
         intros p; rewrite vec_map_map, vec_pos_map.
         apply E2; rewrite E1; auto.
-      + intros s v; simpl.
-        apply fom_eq_rels_full.
+      + intros s v Hs; simpl.
+        apply fom_eq_rels_full; auto.
         intros p; rewrite vec_map_map, vec_pos_map.
         apply E2; rewrite E1; auto.
     Qed.
@@ -198,40 +202,89 @@ Section model_equiv.
            (X : Type) (M : fo_model Σ X) 
            (Y : Type) (K : fo_model Σ Y) 
            (i : X -> Y) (j : Y -> X) (E : forall x, i (j x) = x)
-           (Hs : forall s v, i (fom_syms M s v) = fom_syms K s (vec_map i v))
-           (Hr : forall s v, fom_rels M s v <-> fom_rels K s (vec_map i v)).
+           (ls : list (syms Σ))
+           (lr : list (rels Σ))
+           (Hs : forall s v, In s ls -> i (fom_syms M s v) = fom_syms K s (vec_map i v))
+           (Hr : forall s v, In s lr -> fom_rels M s v <-> fom_rels K s (vec_map i v)).
+
+  Theorem fo_model_term_eq t phi psi :
+           (forall n, i (phi n) = psi n) 
+        -> incl (fo_term_syms t) ls
+        -> i (fo_term_sem (fom_syms M) phi t) 
+         = fo_term_sem (X := nat) (fom_syms K) psi t.
+  Proof.
+    intros H.
+    induction t as [ k | s w Hw ]; intros Hls; rew fot; auto.
+    rewrite Hs.
+    2: { apply Hls; rew fot; simpl; auto. }
+    rewrite vec_map_map.
+    f_equal.
+    apply vec_map_ext.
+    intros t Ht; apply Hw; auto.
+    apply incl_tran with (2 := Hls).
+    rew fot.
+    intros u Hu; right.
+    apply in_flat_map.
+    exists t; split; auto.
+    apply in_vec_list; auto.
+  Qed.
 
   Theorem fo_model_project_equiv A phi psi :
            (forall n, i (phi n) = psi n) 
+        -> incl (fol_syms A) ls
+        -> incl (fol_rels A) lr
         -> fol_sem M phi A <-> fol_sem K psi A.
   Proof.
     revert phi psi.
-    induction A as [ | s | b A HA B HB | q A HA ]; try (simpl; tauto); intros phi psi E'.
+    induction A as [ | r | b A HA B HB | q A HA ]; try (simpl; tauto); intros phi psi E' Hls Hlr.
     + simpl; rewrite Hr, vec_map_map.
       match goal with |- ?x <-> ?y => cut (x = y); [ intros ->; tauto | ] end.
-      f_equal; apply vec_map_ext; intros t _; clear s v.
-      induction t as [ k | s v ]; rew fot; auto.
-      rewrite Hs, vec_map_map; f_equal.
-      apply vec_map_ext; auto.
-    + apply fol_bin_sem_ext; auto.
+      f_equal; apply vec_map_ext; intros t Ht.
+      2: apply Hlr; simpl; auto.
+      apply fo_model_term_eq; auto.
+      apply in_vec_list in Ht.
+      intros s H; apply Hls; simpl.
+      apply in_flat_map.
+      exists t; auto.
+    + simpl; apply fol_bin_sem_ext.
+      * apply HA; auto.
+        - apply incl_tran with (2 := Hls); simpl.
+          intros ? ?; apply in_or_app; auto.
+        - apply incl_tran with (2 := Hlr); simpl.
+          intros ? ?; apply in_or_app; auto.
+      * apply HB; auto.
+        - apply incl_tran with (2 := Hls); simpl.
+          intros ? ?; apply in_or_app; auto.
+        - apply incl_tran with (2 := Hlr); simpl.
+          intros ? ?; apply in_or_app; auto.
     + destruct q; simpl; split.
       * intros (x & Hx).
         exists (i x).
         revert Hx; apply HA.
-        intros []; simpl; auto.
+        - intros []; simpl; auto.
+        - apply incl_tran with (2 := Hls), incl_refl.
+        - apply incl_tran with (2 := Hlr), incl_refl.
       * intros (y & Hy).
         exists (j y).
         revert Hy; apply HA.
-        intros []; simpl; auto.
+        - intros []; simpl; auto.
+        - apply incl_tran with (2 := Hls), incl_refl.
+        - apply incl_tran with (2 := Hlr), incl_refl.
       * intros H y. 
         generalize (H (j y)); apply HA.
-        intros []; simpl; auto.
+        - intros []; simpl; auto.
+        - apply incl_tran with (2 := Hls), incl_refl.
+        - apply incl_tran with (2 := Hlr), incl_refl.
       * intros H x. 
         generalize (H (i x)); apply HA.
-        intros []; simpl; auto.
+        - intros []; simpl; auto.
+        - apply incl_tran with (2 := Hls), incl_refl.
+        - apply incl_tran with (2 := Hlr), incl_refl.
   Qed.
 
 End model_equiv.
+
+Check fo_model_project_equiv.
 
 Section discrete_removal.
 
@@ -240,17 +293,20 @@ Section discrete_removal.
       and decidable model implies satisfiability of A in a finite, decidable
       and discrete model, in fact in a model based on the finite type (pos n) *)
 
-  Theorem fo_discrete_removal Σ (Hs : finite_t (syms Σ)) (Hr : finite_t (rels Σ)) A :
+  Theorem fo_discrete_removal Σ A :
              @fo_form_fin_dec_SAT Σ A
           -> (exists n, @fo_form_fin_discr_dec_SAT_in Σ A (pos n)).
   Proof.
     intros (X & M & Hfin & Hdec & phi & HA).
-    destruct (fo_fin_model_discretize Hs Hr Hfin Hdec)
+    set (ls := fol_syms A).
+    set (lr := fol_rels A).
+    destruct (fo_fin_model_discretize ls lr Hfin Hdec)
       as (n & Md & Mdec & i & j & E1 & E2 & E3).
     set (psy n := i (phi n)).
     exists n, (@pos_eq_dec _), Md, (finite_t_pos _) , Mdec, psy.
     revert HA.
-    apply fo_model_project_equiv with (1 := E1); auto.
+    apply fo_model_project_equiv with (1 := E1) (ls := ls) (lr := lr); 
+      unfold lr, ls; auto; apply incl_refl.
   Qed.
 
 End discrete_removal.
@@ -259,13 +315,11 @@ Check fo_discrete_removal.
 Print Assumptions fo_discrete_removal.
 
 Theorem fo_form_fin_dec_SAT_fin_discr_dec Σ A :
-            finite_t (syms Σ)
-         -> finite_t (rels Σ)
-         -> @fo_form_fin_dec_SAT Σ A 
+            @fo_form_fin_dec_SAT Σ A 
          -> fo_form_fin_discr_dec_SAT A.
 Proof.
-  intros Hs Hr H.
-  destruct fo_discrete_removal with (3 := H) (A := A)
+  intros H.
+  destruct fo_discrete_removal with (1 := H) (A := A)
     as (n & Hn); auto.
   exists (pos n); auto.
 Qed.
