theories/TRAKHTENBROT/reductions.v
@@ -46,21 +46,20 @@ End BPCP_fo_fin_dec_SAT.
 Check BPCP_FIN_DEC_SAT.
 Print Assumptions BPCP_FIN_DEC_SAT.
 
-Section fin_dec_SAT_fin_discr_dec_SAT.
+(** The reduction is the identity here !! *)
 
-  Variable (Σ : fo_signature)
-           (Hs : finite_t (syms Σ)) 
-           (Hr : finite_t (rels Σ)).
+Theorem fo_form_fin_dec_SAT_discr_equiv Σ A : 
+    @fo_form_fin_dec_SAT Σ A <-> @fo_form_fin_discr_dec_SAT Σ A.
+Proof.
+  split.
+  + apply fo_form_fin_dec_SAT_fin_discr_dec.
+  + apply fo_form_fin_discr_dec_SAT_fin_dec.
+Qed.
 
-  Theorem FIN_DEC_SAT_FIN_DISCR_DEC_SAT : @fo_form_fin_dec_SAT Σ ⪯ @fo_form_fin_discr_dec_SAT Σ.
-  Proof.
-    exists (fun A => A); intros A; split.
-    + intros H; destruct fo_discrete_removal with (3 := H) as (n & Hn); auto.
-      exists (pos n); auto.
-    + apply fo_form_fin_discr_dec_SAT_fin_dec.
-  Qed.
+Check fo_form_fin_dec_SAT_discr_equiv.
 
-End fin_dec_SAT_fin_discr_dec_SAT.
+Corollary FIN_DEC_SAT_FIN_DISCR_DEC_SAT Σ : @fo_form_fin_dec_SAT Σ ⪯ @fo_form_fin_discr_dec_SAT Σ.
+Proof. exists (fun A => A); apply fo_form_fin_dec_SAT_discr_equiv. Qed.
 
 Check FIN_DEC_SAT_FIN_DISCR_DEC_SAT.
 Print Assumptions FIN_DEC_SAT_FIN_DISCR_DEC_SAT.
@@ -72,10 +71,7 @@ Theorem FIN_DISCR_DEC_3SAT_FIN_DEC_SAT : @fo_form_fin_discr_dec_SAT (Σrel 3)
 Proof.
   exists Σ3_Σ2_enc; intros A; split.
   + apply SAT3_SAT2.
-  + intros H; apply fo_form_fin_dec_SAT_fin_discr_dec.
-    * exists nil; intros [].
-    * apply finite_t_unit.
-    * apply SAT2_SAT3, H.
+  + intros H; apply fo_form_fin_dec_SAT_fin_discr_dec, SAT2_SAT3, H.
 Qed.
 
 Check FIN_DISCR_DEC_3SAT_FIN_DEC_SAT.
